---
title: "Effect sizes for two means"
author: "Marcello Gallucci"
date: "February 23, 2018"
output: pdf_document
---

```{r setup, include=FALSE}
knitr::opts_chunk$set(echo = TRUE)
```

## Note
why is :
$$\eta_d^2={d^2 \over { 4+d^2}}$$

Followng Wilcox and T.S. Tian (2001), $\sigma_\mu^2={({\Delta \over 2})^2}$ and $\sigma_Y^2=\sigma_\mu^2+\sigma$

INOTE: Cohen 8.2.2 p. 275 is wrong

$$\eta_d^2={\sigma_\mu^2 \over \sigma_Y}={({\Delta \over 2})^2 \over {({\Delta \over 2})^2+\sigma^2}}={{\Delta^2} \over {\Delta^2+4\sigma^2}}$$
thus:
$$1-\eta^2={{4\sigma^2} \over {\Delta^2+4\sigma^2}}$$

and
$${\eta^2 \over {1-\eta^2}}={\Delta^2 \over 4\sigma^2}$$

This is $\omega^2$ from Hays (1988). Taking the square root of it:

$$\sqrt{{\Delta^2 \over 4\sigma^2}}={1 \over 2} d$$
which, by Cohen (1988, p. 276, eq 8.2.5) gives:
$$\sqrt{{\Delta^2 \over 4\sigma^2}}={1 \over 2} d=f$$

We can then write:

$${\eta^2 \over {1-\eta^2}}={{1 \over 4} d^2}$$
which means:

$${\eta^2}={{1 \over 4} d^2 \cdot ({1-\eta^2})}$$

$${\eta^2}={{1 \over 4} d^2 - {1 \over 4} d^2 \eta^2}$$
$${{\eta^2 (4  + d^2)} \over 4}={{1 \over 4} d^2}$$
$$\eta^2={d^2 \over 4  + d^2}$$


## Derived results

### Eta, f and d
$$\sqrt{{\Delta^2 \over 4\sigma^2}}={1 \over 2} d=f={\eta^2 \over {1-\eta^2}}$$

### expected variances

$$\sigma_\mu^2={({\Delta \over 2})^2}$$
and
$$\sigma_Y^2=\sigma_\mu^2+\sigma$$
